Re-implemented CLVM contract-instructions to use first-order stack

execution/CLInterp/CLITranslate.v
@@ -181,8 +181,10 @@ Inductive CInstruction :=
 | CIScale : (list instruction) -> CInstruction
 | CIBoth : CInstruction
 | CITranslate : nat -> CInstruction
+| CITranslateEnd : nat ->  CInstruction
 | CILet : list instruction -> CInstruction
-| CIIf : list instruction -> nat -> CInstruction.
+| CIIf : list instruction -> nat -> CInstruction
+| CIIfEnd : CInstruction.
 
 (** Compilation of CL contracts to CLVM contracts *)
 Fixpoint CompileC (c : Contr) : option (list CInstruction) :=
@@ -191,9 +193,15 @@ Fixpoint CompileC (c : Contr) : option (list CInstruction) :=
   | Transfer p1 p2 a => Some [CITransfer p1 p2 a]
   | Scale e c => do es <- CompileE e; liftM2 List.app (CompileC c) (Some [CIScale (es)])
   | Both c1 c2 => LApp3 (CompileC c2) (CompileC c1) (Some [CIBoth])
-  | Translate n c1 => liftM2 List.app (CompileC c1) (Some [CITranslate n])
-  | If e n c1 c2 => do es <- CompileE e; LApp3 (CompileC c2) (CompileC c1) (Some [CIIf es n])
-  | Let e c => do es <- CompileE e; liftM2 List.app (CompileC c) (Some [CILet es] )
+  | Translate n c1 => do s <- (CompileC c1) ;                                    
+                      (Some ([CITranslate n] ++ s ++ [CITranslateEnd n]))
+  | If e n c1 c2 => do es <- CompileE e;
+                   do s1 <- CompileC c1;
+                   do s2 <- CompileC c2;
+                   Some ([CIIf es n] ++ s2 ++ s1 ++ [CIIfEnd])
+  | Let e c => do es <- CompileE e;
+              do s <- CompileC c;
+              Some ([CILet es] ++ s)
   end.
 
 Definition pop (l : list (Env -> ExtMap -> option Val)) (env : Env) (ext : ExtMap) :=
@@ -310,37 +318,67 @@ Fixpoint StackEInterp (instrs : list instruction) (stack : list (Env -> ExtMap -
               end
   end.
 
-
-Fixpoint stack_within_sem (c1 c2 : Env -> ExtMap  -> option TraceM) 
-         (expis : list instruction) (i : nat)  (env : Env) (rc : ExtMap) : option TraceM
+Fixpoint stack_within_sem  (expis : list instruction) (i : nat)  (env : Env) (rc : ExtMap) : option (bool * nat)
   := match StackEInterp expis [] env rc false with
-     | Some (BVal true) => c1 env rc 
+     | Some (BVal true) => Some (true, i)
      | Some (BVal false) => match i with
-                            | O => c2 env rc
-                            | S j => liftM (delay_traceM 1) (stack_within_sem c1 c2 expis j env (adv_map 1 rc))
+                            | O => Some (false, i)
+                            | S j => stack_within_sem expis j env (adv_map 1 rc)
                             end
      | _ => None
      end.
 
 (** Definition of semantics for CLVM, parameters are in reverse polish notation *)
-Fixpoint StackCInterp (instrs : list CInstruction) (stack : list (Env -> ExtMap -> option TraceM)) (env : Env) (ext: ExtMap) : option TraceM :=
+Fixpoint StackCInterp (instrs : list CInstruction) (stack : list (option TraceM)) (env : Env) (exts: list ExtMap) (w_stack : list (bool * nat)) : option TraceM :=
   match instrs with
-  | [] => match stack with [res] => res env ext | _ => None end
+  | [] => match stack with [res] => res | _ => None end
   | hd::tl =>
     match hd with
-    | CIZero => StackCInterp tl ((fun e et => Some empty_traceM)::stack) env ext
-    | CITransfer p1 p2 c => StackCInterp tl ((fun e et => Some(singleton_traceM (singleton_transM p1 p2 c 1)))::stack) env ext
-    | CIScale expis => match stack with hd2::tl2 => StackCInterp tl ((fun e et => do z <- liftM toZ (StackEInterp expis [] e et false); liftM2 scale_traceM z (hd2 e et))::tl2) env ext
+    | CIZero => StackCInterp tl ((Some empty_traceM)::stack) env exts w_stack
+    | CITransfer p1 p2 c => StackCInterp tl ((Some (singleton_traceM (singleton_transM p1 p2 c 1)))::stack) env exts w_stack
+    | CIScale expis => match stack with hd2::tl2 => do et <- hd_error exts;
+                                                 let trace :=
+                                                     (do z <- liftM toZ (StackEInterp expis [] env et false); liftM2 scale_traceM z hd2)
+                                                 in StackCInterp tl (trace::tl2) env exts w_stack
                                    | [] => None
                        end
-    | CIBoth => match stack with t1::t2::tl2 => StackCInterp tl ((fun e et => liftM2 add_traceM (t1 e et) (t2 e et))::tl2) env ext | _ => None end 
-    | CITranslate n => match stack with t1::tl2 => StackCInterp tl ((fun e et => liftM (delay_traceM n) (t1 e (adv_map (Z.of_nat n) et)))::tl2) env ext | _ => None end
-    | CIIf expis n => match stack with t1::t2::tl2 => StackCInterp tl ((fun e et => stack_within_sem t1 t2 expis n e et)::tl2) env ext | _ => None end
-    | CILet expis => match stack with t1::tl2
-                                      => StackCInterp tl
-                                                      ((fun e et => do v <- (StackEInterp expis [] e et false);(t1 (v::e) et))::tl2)
-                                                      env ext
-                                 | _ => None end
+    | CIBoth => match stack with t1::t2::tl2 =>
+                                let trace := (liftM2 add_traceM t1 t2) in
+                                StackCInterp tl (trace::tl2) env exts w_stack
+                           | _ => None end
+    | CITranslate n  => do et <- hd_error exts;
+                       let et' := (adv_map (Z.of_nat n) et) in
+                       StackCInterp tl stack env (et'::exts) w_stack
+    | CITranslateEnd n => match stack with t::tl2 => match exts with
+                                                    et::exts' => do t' <- t; StackCInterp tl (Some(delay_traceM n t')::tl2) env exts' w_stack
+                                                  | _ => None
+                                                  end
+                                     | _ => None
+                         end
+    | CILet expis => do et <- hd_error exts;
+                     do v <- (StackEInterp expis [] env et false);
+                       StackCInterp tl stack (v::env) exts w_stack
+    | CIIf expis n => match exts with | et::exts' =>
+                                       do w <- stack_within_sem expis n env et;
+                                       let (branch, d_left) := w in
+                                       let d_passed := (n - d_left)%nat in
+                                       let et' := adv_map (Z.of_nat d_passed) et in
+                                       StackCInterp tl stack env (et'::exts') ((branch, d_passed)::w_stack)
+                                | _ => None
+                     end
+    | CIIfEnd => match stack with
+                | t1::t2::tl2 => match w_stack with
+                              | w::w_stack' => 
+                                let (branch, d_passed) := w in
+                                do t1' <- t1;
+                                do t2' <- t2;
+                                 let trace := delay_traceM d_passed (if branch then t1' else t2') in
+                                 StackCInterp tl ((Some trace)::tl2) env (List.tl exts) w_stack'
+                              | _ => None
+                              end
+                | _ => None
+                end
+                                 
     end
   end.
 
@@ -406,7 +444,7 @@ Qed.
 (** This is a proof for one case of Op-expressions. In principle i could just copy this 16 times, with a small correction to the asssertion,
     and a the number of destructs for args. But that is way way too messy. So i need some way to refactor this into cleaner steps.
     It might be worth it to look into the CL repository for already existing tactics.
- destruct op.
+ destruct op. 
          + inversion H1. destruct args. discriminate. destruct args. discriminate. destruct args.
            unfold LApp3 in H4. unfold liftM3 in H4. destruct (CompileE e0) eqn:Eq1. destruct (CompileE e) eqn:Eq2.
            cbn in H4. unfold app3 in H4.  inversion H4. apply all_apply'' in H. destruct H.
@@ -421,23 +459,22 @@ Qed.
         match E[| e|] e1 (ExtMap_to_ExtEnv et) with
         | Some v1 =>
             match E[| e0|] e1 (ExtMap_to_ExtEnv et) with
-            | Some v2 => Some (v1, v2, stack)
+            | Some v2 => Some (v1, v2)
             | None => None
             end
         | None => None
         end
       with
-      | Some (ZVal z1, BVal _, _) => None
-      | Some (ZVal z1, ZVal z2, _) => Some (ZVal (z1 + z2))
+      | Some (ZVal z1, BVal _) => None
+      | Some (ZVal z1, ZVal z2) => Some (ZVal (z1 + z2))
       | _ => None
       end) = (fun (env1 : Env) (ext2 : ExtMap) =>
       do x <-
       liftM2 (fun (x' : Val) (xs' : list Val) => x' :: xs')
         (E[| e|] env1 (ExtMap_to_ExtEnv ext2))
         (liftM2 (fun (x' : Val) (xs' : list Val) => x' :: xs')
-           (E[| e0|] env1 (ExtMap_to_ExtEnv ext2)) 
-           (Some [])); OpSem Add x)).
-            apply functional_extensionality. intro. apply functional_extensionality. intro.
+           (E[| e0|] env1 (ExtMap_to_ExtEnv ext2)) (Some [])); OpSem Add x)).
+            repeat (apply functional_extensionality ; intro). 
              destruct (E[| e|] x (ExtMap_to_ExtEnv x0)) eqn:Eq5.
              destruct (E[| e0|] x (ExtMap_to_ExtEnv x0)) eqn:Eq6; reflexivity.
              reflexivity.
@@ -446,16 +483,13 @@ Qed.
                             apply Eq1. reflexivity. discriminate. discriminate. discriminate.
 *)
 
-Lemma AdvanceMapSound : forall (ext: ExtMap) (d i: Z) (l : ObsLabel),
-FMap.find (l,d + i) ext = FMap.find (l,i) (adv_map d ext).
-Proof. Admitted.
   
 Lemma AdvanceMap1 : forall (ext: ExtMap) (d : Z),
     adv_ext d (ExtMap_to_ExtEnv ext)  = ExtMap_to_ExtEnv (adv_map d ext).
 Proof.
   intros. unfold ExtMap_to_ExtEnv. unfold adv_ext.
   repeat (apply functional_extensionality; intros).
-  rewrite AdvanceMapSound. reflexivity.
+  rewrite AdvanceMapSound. reflexivity. apply x0.
 Qed.
 
 
@@ -464,7 +498,8 @@ Lemma TranlateExpressionStep : forall (e : Exp) (env : Env) (extM : ExtMap) (exp
     expis = l0 ++ l1 -> CompileE e = Some l0 -> (fun env1 ext2 => Esem e env1 (ExtMap_to_ExtEnv ext2)) = f -> 
     StackEInterp (l0 ++ l1) stack env extM false =  StackEInterp l1 (f::stack) env extM false.
 Proof. intro. induction e using Exp_ind'; intros.
-       - destruct op. 
+       - destruct op; inversion H1; try destruct args; try discriminate; try destruct args; try discriminate; try destruct args; try discriminate.
+
        - inversion H0. cbn. cbn in H1. unfold ExtMap_to_ExtEnv in H1.
          unfold find_default. rewrite H1. reflexivity.
        - inversion H0. cbn. cbn in H1. rewrite <- H1.
@@ -520,6 +555,7 @@ Qed.
 Definition vmC (instrs : list CInstruction) (env: Env) (ext: ExtMap) : option TraceM :=
   StackCInterp instrs [] env ext.
 
+
 Definition vmPartial (instrs : list CInstruction) (env: Env) (ext: ExtMap) : option TraceM :=
   StackCPartial instrs [] env ext.
 
@@ -553,3 +589,24 @@ Definition traceMtoTrace (t : TraceM) (default: Z) : Trace :=
                 | Some z => z
                 | None => default
                 end.
+
+Definition option_traceM_to_Trace (t : option TraceM) (default: Z) : option Trace :=
+  liftM2 traceMtoTrace t (Some 0).
+
+
+(*
+Lemma TranlateContractStep : forall (c : Contr) (env : Env) (extM : ExtMap) (instrs l0 l1 : list CInstruction)
+                                 (stack : list (Env -> ExtMap -> option TraceM) ) (t: Env -> ExtMap -> option TraceM),
+    instrs = l0 ++ l1 -> CompileC c = Some l0 -> (forall env1 ext2, Csem c env1 (ExtMap_to_ExtEnv ext2) =
+                                                option_traceM_to_Trace (t env1 ext2) 0) -> 
+    StackCInterp (l0 ++ l1) stack env extM = StackCInterp l1 (t::stack) env extM .
+Proof.
+  intro. induction c; intros.
+  - inversion H0. cbn in *. assert (H5: t = (fun (_ : Env) (_ : ExtMap) => Some empty_traceM)).
+  
+      
+Theorem TranslateContractSound : forall (c : Contr) (e : Env) (ext : ExtMap) (instrs : list CInstruction) ,
+    CompileC c = Some instrs -> Csem c e (ExtMap_to_ExtEnv ext) = do traceM <- (vmC instrs e ext); Some (traceMtoTrace traceM 0).
+Proof.
+  intros. unfold vmC. rewrite (app_nil_end instrs). 
+*)
